templates/multicopy/multicopy_client_level.v
@@ -19,9 +19,9 @@ Definition search' : val :=
   λ: "k",
     let: "t_id" := NewProph in
     let: "p" := NewProph in
-    let: "t'" := search "k" in
-    resolve_proph: "p" to: "t'";;
-    "t'".  
+    let: "vt'" := search "k" in
+    resolve_proph: "p" to: "vt'";;
+    "vt'".  
 
 Section multicopy_client_level.
   Context {Σ} `{heapG Σ, !multicopyG Σ}.
@@ -29,21 +29,21 @@ Section multicopy_client_level.
 
   (** Low-level specs of multicopy operations *)
 
-  Parameter search_recency: ∀ N γ_te γ_he γ_s Prot Inv_tpl k t0, 
+  Parameter search_recency: ∀ N γ_te γ_he γ_s Prot Inv_tpl k v0 t0, 
     ⊢ ⌜k ∈ KS⌝ -∗ 
         mcs_inv N γ_te γ_he γ_s Prot Inv_tpl -∗
-          SR γ_s (k, t0) -∗
+          SR γ_s (k, v0, t0) -∗
               <<< True >>> 
                   search #k @ ⊤ ∖ ↑(mcsN N)
-              <<< ∃ (t': nat), SR γ_s (k, t') ∗ ⌜t0 ≤ t'⌝ , RET #t' >>>.
+              <<< ∃ (v: V) (t: TS), SR γ_s (k, v, t) ∗ ⌜t0 ≤ t⌝ , RET (#v, #t) >>>.
 
-  Parameter upsert_spec: ∀ N γ_te γ_he γ_s Prot Inv_tpl k,
+  Parameter upsert_spec: ∀ N γ_te γ_he γ_s Prot Inv_tpl k (v: V),
     ⊢ ⌜k ∈ KS⌝ -∗ 
         (ghost_update_protocol N γ_te γ_he Prot k) -∗ 
           mcs_inv N γ_te γ_he γ_s Prot Inv_tpl -∗
               <<< ∀ t H, MCS γ_te γ_he t H >>> 
-                     upsert #k @ ⊤ ∖ (↑(mcsN N))
-              <<< MCS γ_te γ_he (t + 1) (H ∪ {[(k,t)]}), RET #() >>>.
+                     upsert #k #v @ ⊤ ∖ (↑(mcsN N))
+              <<< MCS γ_te γ_he (t + 1) (H ∪ {[(k, v, t)]}), RET #() >>>.
                 
   (** Proof of high-level specs for multicopy opeartions *)                
 
@@ -52,36 +52,36 @@ Section multicopy_client_level.
       mcs_inv N γ_te γ_he γ_s (Prot_help N γ_te γ_he γ_td γ_ght) Inv_tpl -∗ 
           <<< ∀ t H, MCS γ_te γ_he t H >>>
                 search' #k @ ⊤ ∖ (↑(mcsN N) ∪ ↑(threadN N))
-          <<<  ∃ (t': nat), MCS γ_te γ_he t H 
-                            ∗ ⌜map_of_set H !!! k = t'⌝, RET #t' >>>.
+          <<<  ∃ (vt: V * TS), MCS γ_te γ_he t H 
+                            ∗ ⌜map_of_set H !!! k = vt⌝, RET (#vt.1, #vt.2) >>>.
   Proof.
     iIntros "% #HInv" (Φ) "AU". wp_lam.
     rename H0 into k_in_KS.
     wp_apply wp_new_proph1; try done.
     iIntros (tid vt)"Htid". wp_pures.
-    wp_apply (typed_proph_wp_new_proph1 NatTypedProph); first done.
-    iIntros (tp p)"Hproph". wp_pures. 
+    wp_apply (typed_proph_wp_new_proph1 VTTypedProph); first done.
+    iIntros (vtp p)"Hproph". wp_pures. 
     iApply fupd_wp.
     iInv "HInv" as (T0 H0) "(mcs_high & Htpl)".
-    iDestruct "mcs_high" as "(>MCS_auth & >HH & >Hist & >MaxTS & Prot)".
-    iAssert (⌜∃ t0, ((k,t0) ∈ H0 ∧ (∀ t, (k,t) ∈ H0 → t ≤ t0) 
-                ∧ map_of_set H0 !! k = Some t0)⌝)%I as "%".
+    iDestruct "mcs_high" as "(>MCS_auth & >HH & >Hist & >MaxTS & >Uniq & Prot)".
+    iAssert (⌜∃ v0 t0, ((k, v0, t0) ∈ H0 ∧ (∀ v t, (k, v, t) ∈ H0 → t ≤ t0) 
+                ∧ map_of_set H0 !! k = Some (v0, t0))⌝)%I as "%".
     { pose proof (map_of_set_lookup_cases H0 k) as H'.
       destruct H' as [H' | H']; try done.
       iDestruct "Hist" as %Hist.
       destruct H' as [H' _].
-      pose proof H' 0 as H'.
+      pose proof H' 0%Z 0 as H'.
       pose proof Hist k k_in_KS as Hist.
       contradiction. }
 
-    destruct H1 as [t0 [kt0_in_H [Max_t0 H_k]]].
-    iMod (own_update γ_s (● H0) (● H0 ⋅ ◯ {[(k,t0)]}) with "[$HH]") as "HH".
-    { apply (auth_update_frac_alloc _ H0 ({[(k,t0)]})).
+    destruct H1 as [v0 [t0 [kt0_in_H [Max_t0 H_k]]]].
+    iMod (own_update γ_s (● H0) (● H0 ⋅ ◯ {[(k, v0, t0)]}) with "[$HH]") as "HH".
+    { apply (auth_update_frac_alloc _ H0 ({[(k, v0, t0)]})).
       apply gset_included. clear -kt0_in_H. set_solver. }
     iDestruct "HH" as "(HH & #mcs_sr)".
                      
-    destruct (decide (tp ≤ t0)).
-    - assert ((tp < t0) ∨ tp = t0) as H' by lia.
+    destruct (decide (vtp.2 ≤ t0)).
+    - assert ((vtp.2 < t0) ∨ vtp.2 = t0) as H' by lia.
       destruct H' as [Hcase' | Hcase'].
       + iModIntro. iSplitR "AU Hproph".
         iNext; iExists T0, H0; iFrame.
@@ -89,21 +89,22 @@ Section multicopy_client_level.
         awp_apply search_recency; try done.
         iAaccIntro with ""; try done.
         { iIntros "_". iModIntro; try eauto with iFrame. } 
-        iIntros (t) "(Hkt & %)". rename H1 into t0_le_t.
+        iIntros (v t) "(Hkt & %)". rename H1 into t0_le_t.
         iModIntro. wp_pures.
-        wp_apply (typed_proph_wp_resolve1 NatTypedProph with "Hproph"); try done.
+        wp_apply (typed_proph_wp_resolve1 VTTypedProph with "Hproph"); try done.
         wp_pures. iModIntro. iIntros "%". rename H1 into tp_eq_t.
-        clear -tp_eq_t Hcase' t0_le_t. exfalso; lia.
+        clear -tp_eq_t Hcase' t0_le_t. rewrite tp_eq_t in Hcase'.
+        simpl in Hcase'. exfalso; lia.
       + iMod "AU" as (T' H') "[MCS [_ Hcomm]]".
         set_solver.
         iAssert (⌜T' = T0 ∧ H' = H0⌝)%I as "%". 
         { iPoseProof (MCS_agree with "[$MCS_auth] [$MCS]") as "(% & %)".
           by iPureIntro. }
         destruct H1 as [H'' H''']. subst T' H'.
-        assert (map_of_set H0 !!! k = t0) as M_k.
+        assert (map_of_set H0 !!! k = (v0, t0)) as M_k.
         { rewrite lookup_total_alt. rewrite H_k.
           by simpl. }
-        iSpecialize ("Hcomm" $! t0). 
+        iSpecialize ("Hcomm" $! (v0, t0)). 
         iMod ("Hcomm" with "[MCS]") as "HΦ".
         { iFrame. by iPureIntro. } 
         iModIntro. iSplitR "HΦ Hproph".
@@ -112,14 +113,32 @@ Section multicopy_client_level.
         awp_apply search_recency without "HΦ"; try done.
         iAaccIntro with ""; try done.
         { iIntros "_". iModIntro; try eauto with iFrame. } 
-        iIntros (t) "(Hkt & %)". rename H1 into t0_le_t.
+        iIntros (v t) "(#Hkt & %)". rename H1 into t0_le_t.
         iModIntro. iIntros "HΦ". wp_pures.
-        wp_apply (typed_proph_wp_resolve1 NatTypedProph with "Hproph"); try done.
+        wp_apply (typed_proph_wp_resolve1 VTTypedProph with "Hproph"); try done.
         wp_pures. iModIntro. iIntros "%". rename H1 into tp_eq_t. 
-        wp_pures. iModIntro.
-        assert (tp = t) as H' by lia.
-        rewrite <-H'. by rewrite Hcase'.
-    - assert (tp > t0) by lia. rename H1 into tp_gr_t0.
+        wp_pures.
+        iInv "HInv" as (T1 H1) "(mcs_high & Htpl)".
+        iDestruct "mcs_high" as "(>MCS_auth & >HH & >Hist & >MaxTS & >Uniq & Prot)".
+        iDestruct "Uniq" as %Uniq.
+        iPoseProof (auth_own_incl γ_s H1 _ with "[$HH $mcs_sr]") as "%".
+        rename H2 into vt0_sub_H1.
+        apply gset_included in vt0_sub_H1.
+        assert ((k,v0,t0) ∈ H1) as vt0_in_H1 by set_solver.
+        iPoseProof (auth_own_incl γ_s H1 _ with "[$HH $Hkt]") as "%".
+        rename H2 into vt_sub_H1.
+        apply gset_included in vt_sub_H1.
+        assert ((k,v,t) ∈ H1) as vt_in_H1 by set_solver.
+        iModIntro. iSplitR "HΦ".
+        iNext; iExists T1, H1; iFrame"∗%". iModIntro.
+        
+        assert (vtp.2 = t) as H'.
+        { rewrite tp_eq_t. simpl. by lia. }
+        rewrite <-H'. rewrite Hcase'.
+        rewrite <-H' in vt_in_H1; rewrite Hcase' in vt_in_H1.
+        pose proof Uniq k v0 v t0 vt0_in_H1 vt_in_H1 as Uniq.
+        by rewrite Uniq.
+    - assert (vtp.2 > t0) by lia. rename H1 into tp_gr_t0.
       iDestruct "Prot" as (R hγt)"(>HR & >Hγt 
                                       & >Domm_hγt & Hstar_reg)".
       iAssert (▷ (⌜tid ∉ R⌝ 
@@ -165,12 +184,12 @@ Section multicopy_client_level.
                   
       iDestruct (laterable with "AU") as (AU_later) "[AU #AU_back]".
       iMod (own_alloc (Excl ())) as (γ_tk') "Token"; first try done.
-      assert ((k,tp) ∉ H0) as ktp_notin_H. 
-      { destruct (decide ((k, tp) ∈ H0)); try done.
-        pose proof Max_t0 tp e as H'.
+      assert (∀ v, (k, v, vtp.2) ∉ H0) as ktp_notin_H. 
+      { intros v. destruct (decide ((k, v, vtp.2) ∈ H0)); try done.
+        pose proof Max_t0 v vtp.2 e as H'.
         clear -H' tp_gr_t0. lia. } 
       iMod (inv_alloc (threadN N) _
-              (∃ H, State γ_sy tid γ_tk' AU_later (Φ) H k tp) 
+              (∃ H, State γ_sy tid γ_tk' AU_later (Φ) H k vtp) 
                                     with "[AU Hreg_sy1]") as "#HthInv".
       { iNext. iExists H0. iFrame "Hreg_sy1". iLeft. 
         unfold Pending. iFrame. by iPureIntro. }
@@ -183,7 +202,7 @@ Section multicopy_client_level.
       rewrite Domm_hγt. clear; set_solver.
       rewrite (big_sepS_delete _ (R ∪ {[tid]}) tid); last by set_solver.
       iSplitR "Hstar_reg". unfold Reg.
-      iExists AU_later, Φ, k, tp, vt, γ_tk', γ_sy. iFrame "∗#".
+      iExists AU_later, Φ, k, vtp, vt, γ_tk', γ_sy. iFrame "∗#".
       assert ((R ∪ {[tid]}) ∖ {[tid]} = R) as H' 
                   by (clear -tid_notin_R; set_solver).
       by rewrite H'.
@@ -191,14 +210,14 @@ Section multicopy_client_level.
       iModIntro. awp_apply search_recency; try done.
       iAaccIntro with ""; try done.
       { iIntros "_". iModIntro; try eauto with iFrame. } 
-      iIntros (t) "(#Hkt & %)". rename H1 into t0_le_t.
+      iIntros (v t) "(#Hkt & %)". rename H1 into t0_le_t.
       iModIntro. wp_pures.
-      wp_apply (typed_proph_wp_resolve1 NatTypedProph with "Hproph"); try done.
+      wp_apply (typed_proph_wp_resolve1 VTTypedProph with "Hproph"); try done.
       wp_pures. iModIntro. iIntros "%". rename H1 into tp_eq_t.
       iApply fupd_wp.
       iInv "HthInv" as (H1)"(>Hth_sy & Hth_or)".
       iInv "HInv" as (T1 H1') "(mcs_high & Htpl)".
-      iDestruct "mcs_high" as "(>MCS_auth & >HH & >Hist & >MaxTS & Prot)".
+      iDestruct "mcs_high" as "(>MCS_auth & >HH & >Hist & >MaxTS & >Uniq & Prot)".
       iDestruct "Prot" as (R1 hγt1)"(>HR & >Hγt 
                                       & >Domm_hγt & Hstar_reg)".
       iAssert (⌜tid ∈ R1⌝)%I as "%".
@@ -238,14 +257,16 @@ Section multicopy_client_level.
         iSplitR "Hth_sy". iApply "Hstar_reg'".
         iNext. iExists P', Q', k', vp', vt', γ_tk'', γ_sy.
         iFrame "∗#". by iNext. } subst H1'.
-      assert (tp = t) as H' by lia. 
-      iAssert (⌜(k,tp) ∈ H1⌝)%I as "%". 
+      assert (vtp.2 = t) as H' by (rewrite tp_eq_t; simpl; lia). 
+      iAssert (⌜(k, vtp.1, vtp.2) ∈ H1⌝)%I as "%". 
       { iPoseProof (own_valid_2 _ _ _ with "[$HH] [$Hkt]") as "H'".
         iDestruct "H'" as %H''.
         apply auth_both_valid_discrete in H''.
         destruct H'' as [H'' _].
         apply gset_included in H''.
-        rewrite <-H' in H''.
+        rewrite tp_eq_t; simpl.
+        rewrite tp_eq_t in H'; simpl in H'.
+        rewrite H'.
         iPureIntro; clear -H''; set_solver. }
       rename H0 into ktp_in_H1.
       iDestruct "Hth_or" as "[Hth_or | Hth_or]".
@@ -264,15 +285,18 @@ Section multicopy_client_level.
       iNext. iExists H1. iFrame "Hth_sy". 
       iRight. iFrame "∗%".
       
-      iModIntro. wp_pures. by rewrite H'.
+      iModIntro. wp_pures. iModIntro.
+      iEval (rewrite tp_eq_t; simpl) in "Hth_or".
+      assert (Z.to_nat t = t) as Ht by lia.
+      by iEval (rewrite Ht) in "Hth_or".
   Qed.
   
   Lemma search_spec_high N γ_te γ_he γ_s Inv_tpl γ_td γ_ght (k: K) :
   ⊢ ⌜k ∈ KS⌝ -∗ 
       <<< ∀ t M, MCS_high N γ_te γ_he γ_s Inv_tpl γ_td γ_ght t M >>>
             search' #k @ ⊤ ∖ (↑(mcsN N) ∪ ↑(threadN N))
-      <<<  ∃ (t': nat), MCS_high N γ_te γ_he γ_s Inv_tpl γ_td γ_ght t M 
-                        ∗ ⌜M !!! k = t'⌝, RET #t' >>>.
+      <<<  ∃ (vt: V*TS), MCS_high N γ_te γ_he γ_s Inv_tpl γ_td γ_ght t M 
+                        ∗ ⌜M !!! k = vt⌝, RET (#vt.1, #vt.2) >>>.
   Proof.
     iIntros "%" (Φ) "AU". rename H0 into k_in_KS.
     iApply fupd_wp. 
@@ -298,16 +322,16 @@ Section multicopy_client_level.
     by iModIntro.
   Qed.
   
-  Lemma ghost_update_registered (k: K) (T: nat) (N: namespace) 
+  Lemma ghost_update_registered (k: K) (v: V) (T: TS) (N: namespace) 
                 (γ_te γ_he γ_ght: gname) 
-                (H1: gset KT) (R: gset proph_id)  :
-        ⌜map_of_set (H1 ∪ {[k, T]}) !!! k = T⌝ -∗
-           MCS_auth γ_te γ_he (T+1) (H1 ∪ {[(k, T)]}) -∗          
+                (H1: gset KVT) (R: gset proph_id)  :
+        ⌜map_of_set (H1 ∪ {[k, v, T]}) !!! k = (v, T)⌝ -∗
+           MCS_auth γ_te γ_he (T+1) (H1 ∪ {[(k, v, T)]}) -∗          
       ([∗ set] t_id ∈ R, Reg N γ_te γ_he γ_ght H1 t_id) 
         ={⊤ ∖ ↑(mcsN N)}=∗ 
       ([∗ set] t_id ∈ R, Reg N γ_te γ_he γ_ght 
-                                      (H1 ∪ {[(k, T)]}) t_id)
-       ∗ MCS_auth γ_te γ_he (T+1) (H1 ∪ {[(k, T)]}).
+                                      (H1 ∪ {[(k, v, T)]}) t_id)
+       ∗ MCS_auth γ_te γ_he (T+1) (H1 ∪ {[(k, v, T)]}).
   Proof.
     iIntros "H1_k MCS_auth".
     iDestruct "H1_k" as %H1_k.
@@ -320,7 +344,7 @@ Section multicopy_client_level.
     iIntros "(Hx & Hbigstar)". 
     iMod ("HInd" with "[$MCS_auth] Hbigstar") as "(H' & MCS_auth)".
     iFrame "H'".
-    iDestruct "Hx" as (P Q k' vp vt γ_tk γ_sy)
+    iDestruct "Hx" as (P Q k' vtp vt γ_tk γ_sy)
               "(Hreg_proph & Hreg_gh & Hreg_sy & #Pau & #Hthinv)".
     iInv "Hthinv" as (H1')"Hstate".
     iDestruct "Hstate" as "(>Hth_sy & Hstate)".
@@ -335,58 +359,61 @@ Section multicopy_client_level.
     iEval (rewrite <-frac_agree_op) in "H'". 
     iEval (rewrite Qp_half_half) in "H'".
     iMod ((own_update (γ_sy) (to_frac_agree 1 H1) 
-                  (to_frac_agree 1 (H1 ∪ {[(k, T)]}))) with "[$H']") as "H'".
+                  (to_frac_agree 1 (H1 ∪ {[(k, v, T)]}))) with "[$H']") as "H'".
     { apply cmra_update_exclusive. 
       unfold valid, cmra_valid. simpl. unfold prod_valid_instance.
       split; simpl; try done. }
     iEval (rewrite <-Qp_half_half) in "H'".
     iEval (rewrite frac_agree_op) in "H'".  
-    iDestruct "H'" as "(Hreg_sy & Hth_sy)".            
+    iDestruct "H'" as "(Hreg_sy & Hth_sy)".
 
     iDestruct "Hstate" as "[Hpending | Hdone]".
     - iDestruct "Hpending" as "(P & >%)".
       rename H0 into vp_notin_H.
-      destruct (decide ((k', vp) ∈ H1 ∪ {[(k, T)]})).
-      + assert ((k',vp) = (k,T)) as H'. 
+      destruct (decide ((k', vtp.1, vtp.2) ∈ H1 ∪ {[(k, v, T)]})).
+      + assert ((k',vtp.1, vtp.2) = (k, v, T)) as H'. 
         { clear -vp_notin_H e. set_solver. }
-        inversion H'. subst k' vp.
+        inversion H'. subst k'. rename H3 into Hv; rename H4 into Ht. 
+        rewrite Hv Ht.
         iDestruct ("Pau" with "P") as ">AU".
         iMod "AU" as (t H1')"[MCS [_ Hclose]]". set_solver.
-        iAssert (⌜H1' = H1 ∪ {[(k, T)]}⌝)%I as "%".
+        iAssert (⌜H1' = H1 ∪ {[(k, v, T)]}⌝)%I as "%".
         { iPoseProof (MCS_agree with "[$MCS_auth] [$MCS]") as "(% & %)".
           by iPureIntro. } subst H1'.
+        iSpecialize ("Hclose" $! (v,T)).  
         iMod ("Hclose" with "[MCS]") as "HQ".
         { iFrame "%∗". }
         iModIntro. iSplitL "Hth_sy HQ".
-        iNext. iExists (H1 ∪ {[(k, T)]}). iFrame.
-        iRight. iSplitL. iLeft. done.
-        iPureIntro. clear; set_solver.
+        iNext. iExists (H1 ∪ {[(k, v, T)]}). iFrame.
+        iRight. iSplitL. iLeft. rewrite Hv Ht.
+        by iEval (simpl) in "HQ".
+        iPureIntro. rewrite Hv Ht. clear; set_solver.
         iModIntro. iFrame.
-        iExists P, Q, k, T, vt, γ_tk, γ_sy.
+        iExists P, Q, k, vtp, vt, γ_tk, γ_sy.
         iFrame "∗#".
       + iModIntro. iSplitR "Hreg_proph Hreg_sy Hreg_gh MCS_auth".
-        iNext. iExists (H1 ∪ {[(k, T)]}). iFrame.
+        iNext. iExists (H1 ∪ {[(k, v, T)]}). iFrame.
         iLeft. iFrame. by iPureIntro.
         iModIntro. iFrame.             
-        iExists P, Q, k', vp, vt, γ_tk, γ_sy.
+        iExists P, Q, k', vtp, vt, γ_tk, γ_sy.
         iFrame "∗#".
     - iModIntro.
       iSplitR "Hreg_proph Hreg_sy Hreg_gh MCS_auth".
-      iNext. iExists (H1 ∪ {[(k, T)]}). iFrame.
+      iNext. iExists (H1 ∪ {[(k, v, T)]}). iFrame.
       iRight. iDestruct "Hdone" as "(HQ & %)".
       iFrame "HQ". iPureIntro. set_solver.
       iModIntro. iFrame. 
-      iExists P, Q, k', vp, vt, γ_tk, γ_sy.
+      iExists P, Q, k', vtp, vt, γ_tk, γ_sy.
       iFrame "∗#". 
   Qed.  
   
   
-  Lemma upsert_spec_high N γ_te γ_he γ_s Inv_tpl γ_td γ_ght (k: K) :
+  Lemma upsert_spec_high N γ_te γ_he γ_s Inv_tpl γ_td γ_ght (k: K) (v: V):
     ⊢ ⌜k ∈ KS⌝ -∗ 
             <<< ∀ T M, MCS_high N γ_te γ_he γ_s Inv_tpl γ_td γ_ght T M >>> 
-                   upsert #k @ ⊤ ∖ (↑(mcsN N) ∪ ↑(threadN N))
+                   upsert #k #v @ ⊤ ∖ (↑(mcsN N) ∪ ↑(threadN N))
             <<< MCS_high N γ_te γ_he γ_s Inv_tpl γ_td γ_ght 
-                        (T + 1) (<[k := T]> M), RET #() >>>.
+                        (T + 1) (<[k := (v,T)]> M), RET #() >>>.
   Proof.
     iIntros "%" (Φ) "AU". rename H0 into k_in_KS.
     iApply fupd_wp. 
@@ -397,11 +424,11 @@ Section multicopy_client_level.
     iAssert (ghost_update_protocol N γ_te γ_he 
                 (Prot_help N γ_te γ_he γ_td γ_ght) k)%I 
                   as "Ghost_updP".
-    { iIntros (T' H')"H1_k MCS_auth".
+    { iIntros (v' T' H')"H1_k MCS_auth".
       iDestruct "H1_k" as %H1_k.
       iIntros "Prot". 
       iDestruct "Prot" as (R hγt)"(HR & Hγt & Domm_hγt & Hstar_reg)".
-      iMod (ghost_update_registered k T' with 
+      iMod (ghost_update_registered k v' T' with 
               "[] [MCS_auth] [$Hstar_reg]") 
                  as "(Hstar_reg & MCS_auth)"; try done.
       iModIntro. iFrame "MCS_auth".
@@ -412,14 +439,16 @@ Section multicopy_client_level.
     iDestruct "MCS_high" as (H1)"(MCS & M_eq_H & _)".
     iDestruct "M_eq_H" as %M_eq_H.
     iAssert (⌜maxTS T1 H1⌝)%I as %maxTS.
-    { by iDestruct "MCS" as "(_ & _ & %)". }
+    { by iDestruct "MCS" as "(_ & _ & % & _)". }
+    iAssert (⌜unique_val H1⌝)%I as %Uniq.
+    { by iDestruct "MCS" as "(_ & _ & _ & %)". }
     iAaccIntro with "MCS".
     { iIntros "MCS". iModIntro.
       iSplitL; try eauto with iFrame.
       iExists H1; iFrame "∗#%". } 
     iIntros "MCS". 
     iModIntro. iSplitL.
-    iExists (H1 ∪ {[k, T1]}). iFrame "∗#".
+    iExists (H1 ∪ {[k, v, T1]}). iFrame "∗#".
     { iPureIntro. apply symmetry. 
       apply map_of_set_insert_eq; try done.
       apply maxTS. }
