templates/multicopy/multicopy_util.v
@@ -19,282 +19,312 @@ Section multicopy_util.
     by iPureIntro.
   Qed.
 
-  Lemma map_of_set_lookup_cases H1 k:
-        (∃ T, (k, T) ∈ H1 ∧ (∀ t, (k,t) ∈ H1 → t ≤ T) ∧ map_of_set H1 !! k = Some T)
-      ∨ ((∀ t, (k,t) ∉ H1) ∧ map_of_set H1 !! k = None).
+  Lemma map_of_set_lookup_cases H k:
+        (∃ v t, (k, v, t) ∈ H ∧ (∀ v' t', (k, v', t') ∈ H → t' ≤ t) ∧ map_of_set H !! k = Some (v, t))
+      ∨ ((∀ v t, (k, v, t) ∉ H) ∧ map_of_set H !! k = None).
   Proof.
-    set (P := λ (m: gmap K nat) (X: gset KT),
-                (∃ T, (k, T) ∈ X ∧ (∀ t, (k,t) ∈ X → t ≤ T)
-                          ∧ m !! k = Some T)
-              ∨ ((∀ t, (k,t) ∉ X) ∧ m !! k = None)).
+    set (P := λ (m: gmap K (V*TS)) (X: gset KVT),
+                (∃ v t, (k, v, t) ∈ X ∧ (∀ v' t', (k, v', t') ∈ X → t' ≤ t)
+                          ∧ m !! k = Some (v, t))
+              ∨ ((∀ v t, (k, v, t) ∉ X) ∧ m !! k = None)).
     apply (set_fold_ind_L P); try done.
     - unfold P. right. split; try done.
-    - intros [k' t'] X m Hnotin Hp.
+    - intros [[k' v'] t'] X m Hnotin Hp.
       destruct (decide (k' = k)).
       + replace k'. unfold P. left. unfold P in Hp.
         destruct Hp as [Hp | Hp].
-        * destruct Hp as [T Hp].
-          destruct (decide (T < t')).
-          ** exists t'. repeat split; first set_solver.
-             intros t. rewrite elem_of_union.
-             intros [Hv | Hv]. assert (t = t') by set_solver.
+        * destruct Hp as [v [t Hp]].
+          destruct (decide (t < t')).
+          ** exists v', t'. repeat split; first set_solver.
+             intros v'' t''. rewrite elem_of_union.
+             intros [Hv | Hv]. assert (t'' = t') by set_solver.
              lia. destruct Hp as [_ [Hp _]].
-             pose proof Hp t Hv. lia. simpl.
-             assert (m !!! k <= t') as Hm.
+             pose proof Hp v'' t'' Hv. lia. simpl.
+             assert ((m !!! k).2 <= t') as Hm.
              { unfold lookup_total, map_lookup_total.
                destruct Hp as [_ [_ Hp]]. rewrite Hp.
                simpl. lia. }
-             destruct (decide (m !!! k ≤ t')); try done.
+             destruct (decide ((m !!! k).2 ≤ t')); try done.
              by rewrite lookup_insert.
-          ** assert (t' = T ∨ t' < T) as Ht by lia. clear n.
-             exists T. destruct Hp as [Hp1 [Hp2 Hp3]].
-             repeat split; first set_solver.
-             intros t. rewrite elem_of_union.
-             intros [Hv | Hv]. assert (t = t') by set_solver.
-             lia. pose proof Hp2 t Hv. lia. simpl.
-             destruct Ht as [Ht | Ht].
-             assert (m !!! k <= t') as Hm.
-             { unfold lookup_total, map_lookup_total.
-               rewrite Hp3. simpl. lia. }
-             destruct (decide (m !!! k ≤ t')); try done.
-             rewrite lookup_insert. by rewrite Ht.
-             assert (m !!! k > t') as Hm.
-             { unfold lookup_total, map_lookup_total.
-               rewrite Hp3. simpl. lia. }
-             destruct (decide (m !!! k ≤ t')); try done.
-             exfalso. lia.
-        * exists t'. simpl. repeat split; first set_solver.
-          intros t. rewrite elem_of_union. intros [Hv | Hv].
-          assert (t = t') by set_solver. lia.
-          destruct Hp as [Hp _].
-          pose proof Hp t as Hp. set_solver.
-          assert (m !!! k ≤ t') as Hm.
+          ** assert (t' = t ∨ t' < t) as Ht by lia. clear n.
+             destruct Hp as [Hp1 [Hp2 Hp3]].
+             destruct Ht as [Ht | Ht]. 
+             *** replace t'. exists v', t.
+                 repeat split; first set_solver.
+                 intros v'' t''. rewrite elem_of_union.
+                 intros [Hv | Hv]. assert (t'' = t) by set_solver.
+                 assert (v'' = v') by set_solver.
+                 lia. pose proof Hp2 v'' t'' Hv. lia. simpl.
+                 assert ((m !!! k).2 <= t) as Hm.
+                 { unfold lookup_total, map_lookup_total.
+                   rewrite Hp3. simpl. lia. }
+                 destruct (decide ((m !!! k).2 ≤ t)); try done.
+                 rewrite lookup_insert. done.
+             *** exists v, t. repeat split; first set_solver.
+                 intros v'' t''. rewrite elem_of_union.
+                 intros [Hv | Hv]. assert (t'' = t') by set_solver.
+                 assert (v'' = v') by set_solver.
+                 lia. pose proof Hp2 v'' t'' Hv. lia. simpl.
+                 assert (not ((m !!! k).2 ≤ t')) as Hm.
+                 { unfold lookup_total, map_lookup_total.
+                   rewrite Hp3. simpl. lia. }
+                 destruct (decide ((m !!! k).2 ≤ t')); try done.
+        * exists v', t'. simpl. repeat split; first set_solver.
+          intros v'' t''. rewrite elem_of_union. intros [Hv | Hv].
+          assert (t'' = t') by set_solver. assert (v'' = v') by set_solver.
+          lia. destruct Hp as [Hp _].
+          pose proof Hp v'' t'' as Hp. set_solver.
+          assert ((m !!! k).2 ≤ t') as Hm.
           { unfold lookup_total, map_lookup_total.
             destruct Hp as [_ Hp]. rewrite Hp. simpl; lia. }
-          destruct (decide (m !!! k ≤ t')); try done.
+          destruct (decide ((m !!! k).2 ≤ t')); try done.
           by rewrite lookup_insert.
       + unfold P. unfold P in Hp.
         destruct Hp as [Hp | Hp].
-        * destruct Hp as [T [Hp1 [Hp2 Hp3]]].
-          left. exists T. repeat split; first set_solver.
-          intros t Hkt. assert ((k,t) ∈ X) as Hx by set_solver.
-          by pose proof Hp2 t Hx.
-          simpl.
-          destruct (decide (m !!! k' <= t')).
+        * destruct Hp as [v [t [Hp1 [Hp2 Hp3]]]].
+          left. exists v, t. repeat split; first set_solver.
+          intros v'' t'' Hkt. assert ((k, v'', t'') ∈ X) as Hx by set_solver.
+          by pose proof Hp2 v'' t'' Hx. simpl.
+          destruct (decide ((m !!! k').2 <= t')).
           rewrite lookup_insert_ne; try done. done.
         * destruct Hp as [Hp1 Hp2]. right.
           repeat split; first set_solver. simpl.
-          destruct (decide (m !!! k' <= t')).
+          destruct (decide ((m !!! k').2 <= t')).
           rewrite lookup_insert_ne; try done. done.
   Qed.
 
-  Lemma map_of_set_lookup H k T :
-        (k, T) ∈ H → (∀ t, (k, t) ∈ H → t ≤ T) →
-           map_of_set H !! k = Some T.
+  Lemma map_of_set_lookup H k v t :
+        unique_val H → 
+          (k, v, t) ∈ H → (∀ v' t', (k, v', t') ∈ H → t' ≤ t) →
+            map_of_set H !! k = Some (v, t).
   Proof.
-    intros Hkt Hmax.
+    intros Uniq Hkt Hmax.
     pose proof (map_of_set_lookup_cases H k) as Hp.
     destruct Hp as [Hp | Hp].
-    - destruct Hp as [T' [Hp1 [Hp2 Hp3]]].
-      pose proof Hmax T' Hp1 as Ht1.
-      pose proof Hp2 T Hkt as Ht2.
-      assert (T = T') as Ht by lia.
-      by rewrite Ht.
+    - destruct Hp as [v' [t' [Hp1 [Hp2 Hp3]]]].
+      pose proof Hmax v' t' Hp1 as Ht1.
+      pose proof Hp2 v t Hkt as Ht2.
+      assert (t = t') as Ht by lia. subst t'.
+      pose proof Uniq k v v' t Hkt Hp1 as Uniq.
+      by subst v'.
     - destruct Hp as [Hp _].
-      pose proof Hp T. set_solver.
-  Qed.
-
-  Lemma map_of_set_lookup_some_aux (H: gset KT) k :
-          (∀ t, (k,t) ∉ H) ∨ (∃ T, (k, T) ∈ H ∧ (∀ t', (k,t') ∈ H → t' ≤ T)).
+      pose proof Hp v t. set_solver.
+  Qed.  
+  
+  Lemma map_of_set_lookup_some_aux (H: gset KVT) k :
+        unique_val H → 
+          (∀ v t, (k, v, t) ∉ H) ∨ 
+            (∃ v t, (k, v, t) ∈ H ∧ (∀ v' t', (k, v', t') ∈ H → t' ≤ t)).
   Proof.
-    set (P := λ (X: gset KT), (∀ t, (k,t) ∉ X) ∨
-                  (∃ T, (k, T) ∈ X ∧ (∀ t', (k,t') ∈ X → t' ≤ T))).
+    intros Uniq.
+    set (P := λ (X: gset KVT), (∀ v t, (k, v, t) ∉ X) ∨
+                  (∃ v T, (k, v, T) ∈ X ∧ (∀ v' t', (k, v', t') ∈ X → t' ≤ T))).
     apply (set_ind_L P); try done.
-    - unfold P. left. intros t. set_solver.
-    - intros [k' t'] X Hkt HP. subst P.
+    - unfold P. left. intros v t. set_solver.
+    - intros [[k' v'] t'] X Hkt HP. subst P.
       simpl in HP. simpl. destruct (decide (k' = k)).
       + subst k'. destruct HP as [H' | H'].
-        * right. exists t'. split.
-          set_solver. intros t. destruct (decide (t' = t)).
+        * right. exists v', t'. split.
+          set_solver. intros v t. destruct (decide (t' = t)).
           subst t'. intros; done.
-          intros H''. assert ((k,t) ∈ X).
-          set_solver. pose proof H' t as H'.
+          intros H''. assert ((k,v,t) ∈ X).
+          set_solver. pose proof H' v t as H'.
           done.
-        * right. destruct H' as [T H'].
+        * right. destruct H' as [v [T H']].
           destruct (decide (t' < T)).
-          ** exists T. split.
+          ** exists v, T. split.
              destruct H' as [H' _].
-             set_solver. intros t Hkt'.
+             set_solver. intros v'' t'' Hkt'.
              rewrite elem_of_union in Hkt'*; intros Hkt'.
              destruct Hkt' as [Hkt' | Hkt'].
              rewrite elem_of_singleton in Hkt'*; intros Hkt'.
              inversion Hkt'. lia.
-             destruct H' as [_ H'']. apply H''; try done.
-          ** exists t'. split. set_solver.
-             intros t Hkt'. rewrite elem_of_union in Hkt'*; intros Hkt'.
+             destruct H' as [_ H'']. apply (H'' v''); try done.
+          ** exists v', t'. split. set_solver.
+             intros v'' t'' Hkt'. 
+             rewrite elem_of_union in Hkt'*; intros Hkt'.
              destruct Hkt' as [Hkt' | Hkt'].
              rewrite elem_of_singleton in Hkt'*; intros Hkt'.
              inversion Hkt'. lia.
              destruct H' as [_ H''].
              apply (Nat.le_trans _ T _); try lia.
-             apply H''. try done.
+             apply (H'' v''). try done.
       + destruct HP as [H' | H'].
-        * left. intros t. set_solver.
-        * right. destruct H' as [T H'].
-          exists T. destruct H' as [H' H''].
-          split. set_solver. intros t.
+        * left. intros v t. set_solver.
+        * right. destruct H' as [v [T H']].
+          exists v, T. destruct H' as [H' H''].
+          split. set_solver. intros v'' t''.
           intros Hkt'. rewrite elem_of_union in Hkt'*; intros Hkt'.
           destruct Hkt' as [Hkt' | Hkt'].
           rewrite elem_of_singleton in Hkt'*; intros Hkt'.
-          inversion Hkt'. done. apply H''; try done.
+          inversion Hkt'. done. apply (H'' v''); try done.
   Qed.
-
-  Lemma map_of_set_lookup_some (H: gset KT) k t :
-              (k, t) ∈ H → is_Some(map_of_set H !! k).
+  
+  Lemma map_of_set_lookup_some (H: gset KVT) k v t :
+          unique_val H →    
+            (k, v, t) ∈ H → is_Some(map_of_set H !! k).
   Proof.
-    intros Hkt.
-    pose proof map_of_set_lookup_some_aux H k as Hkt'.
+    intros Uniq Hkt.
+    pose proof map_of_set_lookup_some_aux H k Uniq as Hkt'.
     destruct Hkt' as [Hkt' | Hkt'].
-    { pose proof Hkt' t as H'. set_solver. }
+    { pose proof Hkt' v t as H'. set_solver. }
     pose proof (map_of_set_lookup_cases H k) as H'.
     destruct H' as [H' | H'].
-    - destruct H' as [T' H'].
+    - destruct H' as [v' [T' H']].
       destruct H' as [_ [_ H']].
-      rewrite H'. by exists T'.
-    - destruct Hkt' as [T Hkt'].
+      rewrite H'. by exists (v',T').
+    - destruct Hkt' as [v' [T Hkt']].
       destruct Hkt' as [Hkt' _].
       destruct H' as [H' _].
-      pose proof H' T as H'.
+      pose proof H' v' T as H'.
       set_solver.
   Qed.
-
-  Lemma map_of_set_lookup_lb H k t :
-    (k,t) ∈ H → t ≤ map_of_set H !!! k.
-  Proof.
+  
+  Lemma map_of_set_lookup_lb H k v t :
+    (k, v, t) ∈ H → t ≤ (map_of_set H !!! k).2.
+  Proof. 
     intros kt_in_H.
     pose proof map_of_set_lookup_cases H k as [H' | H'].
-    - destruct H' as [T [kT_in_H [H' H_k]]].
+    - destruct H' as [V [T [kT_in_H [H' H_k]]]].
       rewrite lookup_total_alt. rewrite H_k.
-      simpl. apply H'; try done.
+      simpl. apply (H' v); try done.
     - destruct H' as [H' _].
-      pose proof H' t as H'.
+      pose proof H' v t as H'.
       contradiction.
   Qed.
-
-  Lemma set_of_map_member_ne (C: gmap K nat) k :
+  
+  Lemma set_of_map_member_ne (C: gmap K (V*TS)) k :
             C !! k = None →
-              ∀ t, (k, t) ∉ set_of_map C.
-  Proof.
-    set (P := λ (s: gset KT) (m: gmap K nat),
-                   m !! k = None → ∀ t, (k, t) ∉ s).
+              ∀ v t, (k, v, t) ∉ set_of_map C.
+  Proof.  
+    set (P := λ (s: gset KVT) (m: gmap K (V*TS)),
+                   m !! k = None → ∀ v t, (k, v, t) ∉ s).
     apply (map_fold_ind P); try done.
     intros kx tx m r Hm HP. unfold P.
     unfold P in HP. destruct (decide (kx = k)).
     - subst kx. rewrite lookup_insert. try done.
     - rewrite lookup_insert_ne; try done.
       intros Hm'. pose proof HP Hm' as HP.
-      intros t. intros Hnot.
+      intros v t. intros Hnot.
       rewrite elem_of_union in Hnot*; intros Hnot.
       destruct Hnot as [Hnot | Hnot].
       + by apply HP in Hnot.
       + rewrite elem_of_singleton in Hnot*; intros Hnot.
         inversion Hnot. try done.
   Qed.
-
-  Lemma map_of_set_union_ne H k t k' :
-          k' ≠ k → map_of_set (H ∪ {[(k, t)]}) !! k' = map_of_set H !! k'.
+  
+  Lemma map_of_set_union_ne H k v t k' :
+          unique_val H → k' ≠ k → 
+            map_of_set (H ∪ {[(k, v, t)]}) !! k' = map_of_set H !! k'.
   Proof.
-    intros Hk.
+    intros Uniq Hk.
     pose proof (map_of_set_lookup_cases H k') as Hp.
-    pose proof (map_of_set_lookup_cases (H ∪ {[(k,t)]}) k') as Hu.
+    pose proof (map_of_set_lookup_cases (H ∪ {[(k, v, t)]}) k') as Hu.
     destruct Hp as [Hp | Hp].
     - destruct Hu as [Hu | Hu].
-      + destruct Hp as [T [Hp1 [Hp2 Hp3]]].
-        destruct Hu as [T' [Hu1 [Hu2 Hu3]]].
+      + destruct Hp as [v0 [T [Hp1 [Hp2 Hp3]]]].
+        destruct Hu as [v0' [T' [Hu1 [Hu2 Hu3]]]].
         assert (T ≤ T') as Ht1.
-        { assert ((k', T) ∈ H ∪ {[k, t]}) as Ht by set_solver.
-          by pose proof Hu2 T Ht. }
+        { assert ((k', v0, T) ∈ H ∪ {[k, v, t]}) as Ht by set_solver.
+          by pose proof Hu2 v0 T Ht. }
         assert (T' ≤ T) as Ht2.
-        { assert ((k', T') ∈ H) as Ht by set_solver.
-          by pose proof Hp2 T' Ht. }
+        { assert ((k', v0', T') ∈ H) as Ht by set_solver.
+          by pose proof Hp2 v0' T' Ht. }
         rewrite Hp3 Hu3. assert (T = T') as Ht by lia.
-        by rewrite Ht.
-      + destruct Hp as [T [Hp1 [Hp2 Hp3]]].
+        subst T'. assert ((k', v0', T) ∈ H) as H'.
+        { clear -Hu1 Hk; set_solver. }
+        pose proof Uniq k' v0 v0' T Hp1 H' as Uniq.
+        by rewrite Uniq.
+      + destruct Hp as [v0 [T [Hp1 [Hp2 Hp3]]]].
         destruct Hu as [Hu1 Hu2].
-        pose proof Hu1 T as Hu1. set_solver.
+        pose proof Hu1 v0 T as Hu1. set_solver.
     - destruct Hu as [Hu | Hu].
       + destruct Hp as [Hp1 Hp2].
-        destruct Hu as [T' [Hu1 [Hu2 Hu3]]].
-        pose proof Hp1 T' as Hp1. set_solver.
+        destruct Hu as [v0 [T' [Hu1 [Hu2 Hu3]]]].
+        pose proof Hp1 v0 T' as Hp1. set_solver.
       + destruct Hp as [Hp1 Hp2].
         destruct Hu as [Hu1 Hu2].
         by rewrite Hp2 Hu2.
   Qed.
-
-  Lemma map_of_set_insert_eq (C: gmap K nat) k T H :
-        (∀ t, (k, t) ∈ H → t < T) →
-                  C = map_of_set H →
-                 <[k := T]> C = map_of_set (H ∪ {[(k, T)]}).
+  
+  Lemma map_of_set_insert_eq (C: gmap K (V*TS)) k v t H :
+        unique_val H →
+          (∀ v' t', (k, v', t') ∈ H → t' < t) →
+            C = map_of_set H →
+              <[k := (v, t)]> C = map_of_set (H ∪ {[(k, v, t)]}).
   Proof.
-    intros Hmax Hc. apply map_eq. intros k'.
+    intros Uniq Hmax Hc. apply map_eq. intros k'.
     destruct (decide (k' = k)).
     - replace k'. rewrite lookup_insert.
-      rewrite (map_of_set_lookup _ _ T); try done.
-      set_solver. intros t'. rewrite elem_of_union.
-      intros [Hk | Hk]. pose proof Hmax t' Hk. lia.
-      assert (t' = T) by set_solver. by replace t'.
+      rewrite (map_of_set_lookup _ _ v t); try done.
+      { intros k0 v0 v0' t0. rewrite !elem_of_union.
+        intros [Hkvt0 | Hkvt0]; intros [Hkvt0' | Hkvt0'].
+        - by pose proof Uniq k0 v0 v0' t0 Hkvt0 Hkvt0'.
+        - assert ((k0, v0', t0) = (k, v, t)) as H' by set_solver.
+          inversion H'. subst k0 v0' t0.
+          pose proof Hmax v0 t Hkvt0 as Hmax. lia.
+        - assert ((k0, v0, t0) = (k, v, t)) as H' by set_solver.
+          inversion H'. subst k0 v0 t0.
+          pose proof Hmax v0' t Hkvt0' as Hmax. lia.
+        - assert ((k0, v0, t0) = (k0, v0', t0)) as H' by set_solver.
+          by inversion H'. }  
+      set_solver. intros v' t'. rewrite elem_of_union.
+      intros [Hk | Hk]. pose proof Hmax v' t' Hk. lia.
+      assert (t' = t) by set_solver. by replace t'.
     - rewrite map_of_set_union_ne; try done.
       rewrite lookup_insert_ne; try done.
       by rewrite Hc.
   Qed.
-
-  Lemma set_of_map_member (C: gmap K nat) k t :
-            C !! k = Some(t) →
-              (k, t) ∈ set_of_map C.
+  
+  Lemma set_of_map_member (C: gmap K (V*TS)) k v t :
+            C !! k = Some((v, t)) →
+              (k, v, t) ∈ set_of_map C.
   Proof.
     intros Hc. unfold set_of_map.
-    set (P := λ (s: gset KT) (m: gmap K nat),
-                  ∀ j x, m !! j = Some x → (j,x) ∈ s).
+    set (P := λ (s: gset KVT) (m: gmap K (V*TS)),
+                  ∀ j v x, m !! j = Some (v, x) → (j, v, x) ∈ s).
     apply (map_fold_ind P); try done.
     intros i x m s Hmi Hp. unfold P.
-    intros j x'. destruct (decide (i = j)).
+    intros j v' x'. destruct (decide (i = j)).
     - replace j. rewrite lookup_insert.
       intros H'; inversion H'. set_solver.
     - rewrite lookup_insert_ne; try done.
-      pose proof Hp j x' as Hp'. set_solver.
+      pose proof Hp j v' x' as Hp'. set_solver.
   Qed.
-
-  Lemma set_of_map_member_rev (C: gmap K nat) k t :
-            (k, t) ∈ set_of_map C →
-                C !! k = Some(t).
+  
+  Lemma set_of_map_member_rev (C: gmap K (V*TS)) k v t :
+            (k, v, t) ∈ set_of_map C →
+                C !! k = Some((v, t)).
   Proof.
-    set (P := λ (s: gset KT) (m: gmap K nat),
-                  ∀ j x, (j,x) ∈ s → m !! j = Some x).
+    set (P := λ (s: gset KVT) (m: gmap K (V*TS)),
+                  ∀ k v t, (k, v, t) ∈ s → m !! k = Some (v, t)).
     apply (map_fold_ind P); try done.
-    intros i x m r Hmi Hp. unfold P.
-    intros j x'. destruct (decide (i = j)).
-    - replace j. rewrite lookup_insert.
-      rewrite elem_of_union. intros [Hr | Hr].
-      unfold P in Hp. pose proof Hp i x' Hr as Hp.
+    intros k' vt m r Hmi Hp. unfold P.
+    intros k0 v0 t0 Hkvt0. destruct (decide (k0 = k')).
+    - subst k0. rewrite lookup_insert.
+      rewrite elem_of_union in Hkvt0*; intros Hkvt0.
+      destruct Hkvt0 as [Hkvt0 | Hkvt0].
+      unfold P in Hp. pose proof Hp k' v0 t0 Hkvt0 as Hp.
       rewrite Hp in Hmi. inversion Hmi.
-      assert (x = x') by set_solver. by replace x.
-    - intros H'. assert ((j,x') ∈ r) as Hj by set_solver.
-      pose proof Hp j x' Hj as Hp.
+      assert ((v0, t0) = (vt.1, vt.2)) as H' by set_solver.
+      inversion H'. destruct vt as [v' t']; by simpl.
+    - assert ((k0, v0, t0) ∈ r) as Hj by set_solver.
+      pose proof Hp k0 v0 t0 Hj as Hp.
       rewrite lookup_insert_ne; try done.
   Qed.
-
-  Lemma set_of_map_insert_subseteq (C: gmap K nat) k t :
-    set_of_map (<[k := t]> C) ⊆ set_of_map C ∪ {[(k, t)]}.
+  
+  Lemma set_of_map_insert_subseteq (C: gmap K (V*TS)) k v t :
+    set_of_map (<[k := (v, t)]> C) ⊆ set_of_map C ∪ {[(k, v, t)]}.
   Proof.
-    intros [k' t'] Hkt. destruct (decide (k' = k)).
-    - replace k'. rewrite e in Hkt.
-    apply set_of_map_member_rev in Hkt.
-    rewrite lookup_insert in Hkt.
-    inversion Hkt. set_solver.
+    intros [[k' v'] t'] Hkt. destruct (decide (k' = k)).
+    - subst k'.
+      apply set_of_map_member_rev in Hkt.
+      rewrite lookup_insert in Hkt.
+      inversion Hkt. set_solver.
     - apply set_of_map_member_rev in Hkt.
-    rewrite lookup_insert_ne in Hkt; try done.
-    apply set_of_map_member in Hkt.
-    set_solver.
+      rewrite lookup_insert_ne in Hkt; try done.
+      apply set_of_map_member in Hkt.
+      set_solver.
   Qed.
 
 End multicopy_util.
